cava/arrow-examples/UnsignedAdder.v
@@ -1,0 +1,303 @@
+(****************************************************************************)
+(* Copyright 2020 The Project Oak Authors                                   *)
+(*                                                                          *)
+(* Licensed under the Apache License, Version 2.0 (the "License")           *)
+(* you may not use this file except in compliance with the License.         *)
+(* You may obtain a copy of the License at                                  *)
+(*                                                                          *)
+(*     http://www.apache.org/licenses/LICENSE-2.0                           *)
+(*                                                                          *)
+(* Unless required by applicable law or agreed to in writing, software      *)
+(* distributed under the License is distributed on an "AS IS" BASIS,        *)
+(* WITHOUT WARRANTIES OR CONDITIONS OF ANY KIND, either express or implied. *)
+(* See the License for the specific language governing permissions and      *)
+(* limitations under the License.                                           *)
+(****************************************************************************)
+
+From Arrow Require Import Category ClosureConversion.
+From Cava Require Import Arrow.ArrowExport.
+
+From Coq Require Import Strings.String Bvector List NArith Nat Lia Plus.
+Import ListNotations.
+Import EqNotations.
+
+Local Open Scope string_scope.
+
+Section notation.
+  Import KappaNotation.
+
+  Section var.
+    Variable var: Kind -> Kind -> Type.
+
+    Definition rewrite_vector {A x y} (H: x = y)
+      : CavaExpr var << Vector A x, Unit >> <<Vector A y>>
+      :=
+    match PeanoNat.Nat.eq_dec x y with
+    | left Heq =>
+      rew [fun x => CavaExpr var << _, _ >> <<Vector A x>> ] Heq in Id
+    | right Hneq => (ltac:(exfalso;contradiction))
+    end.
+
+    Definition rewrite_kind {x y} (H: x = y)
+      : CavaExpr var << x, Unit >> y
+      :=
+    match decKind x y with
+    | left Heq =>
+      rew [fun x => CavaExpr var << _ >> <<x>> ] Heq in Id
+    | right Hneq => (ltac:(exfalso;contradiction))
+    end.
+
+    Definition unsigned_adder a b c
+    : CavaExpr var << Vector Bit a, Vector Bit b, Unit >> (Vector Bit c) :=
+    <[ \ x y => unsigned_add a b c x y ]>.
+
+    Definition adder3 s1 s2 s3
+    : CavaExpr var << Vector Bit s1, Vector Bit s2, Vector Bit s3, Unit >> (Vector Bit _) :=
+    <[ \ a b c => a + b + c ]>.
+
+    Definition split_pow2 A n
+      : CavaExpr var << Vector A (2^(S n)), Unit >> <<Vector A (2^n), Vector A (2^n)>>.
+      refine (<[\ x => 
+        let '(l,r) = split_at (2^n) x in
+        (l, !(rewrite_vector _) r)
+         ]>);
+      induction n; simpl; auto; nia.
+    Defined.
+
+    Fixpoint tree (A: Kind) (n: nat)
+      (f: CavaExpr var << A, A, Unit >> A) {struct n}
+      : CavaExpr var << Vector A (2^(n+1)), Unit >> A :=
+    match n with
+    | O => <[ \ vec =>
+        let '(a,vec') = uncons vec in
+        let '(b,_) = uncons vec' in
+        !f a b
+      ]>
+    | S n' => 
+      <[\ x =>
+          let '(left,right) = !(split_pow2 A (n'+1)) x in
+          let a = !(tree A n' f) left in
+          let b = !(tree A n' f) right in
+          !f a b
+      ]>
+    end.
+
+    Definition tree_adder a n
+    : CavaExpr var << Vector (Vector Bit a) (2^(n+1)), Unit >> (Vector Bit a) :=
+    <[ \ v => !(tree (Vector Bit a) n (unsigned_adder a a a)) v  ]>.
+
+    Fixpoint dt_tree_fold'
+      (n k: nat)
+      (T: nat -> Kind)
+      (f: forall n, CavaExpr var << T n, T n, Unit >> (T (S n))) {struct n}
+      : CavaExpr var << Vector (T k) (2^(n + 1)), Unit >> (T (S (n + k))) :=
+    match n with
+    | O => 
+      <[ \ vec =>
+        let '(a,vec') = uncons vec in
+        let '(b,_) = uncons vec' in
+        !(rewrite_kind (ltac:(auto))) (!(f k) a b)
+      ]>
+    | S n' =>  
+      <[\ x =>
+          let '(left,right) = !(split_pow2 (T k) (n'+1)) x in
+          let a = !(dt_tree_fold' n' k T f) left in
+          let b = !(dt_tree_fold' n' k T f) right in
+          !(f _) a b
+      ]>
+    end.
+
+    Definition dt_tree_fold
+      (n: nat)
+      (T: nat -> Kind)
+      (f: forall n, CavaExpr var << T n, T n, Unit >> (T (S n))) 
+      : CavaExpr var << Vector (T 0) (2^(n + 1)), Unit >> (T (S n)) :=
+      match PeanoNat.Nat.eq_dec (S (n + 0)) (S n) with
+      | left Heq => rew [fun x => CavaExpr var <<_>> <<T x>> ] Heq in dt_tree_fold' n 0 T f
+      | right Hneq => (ltac:(exfalso; abstract lia))
+      end.
+
+    Lemma max_nn_add_1_is_S_n: forall n, 1 + max n n = S n.
+    Proof. intros; rewrite PeanoNat.Nat.max_id; auto. Qed.
+
+    Definition growth_adder n 
+    : CavaExpr var << Vector Bit n, Vector Bit n, Unit >> (Vector Bit (S n)) :=
+    <[ \ a b => !(rewrite_vector (max_nn_add_1_is_S_n _)) (a + b) ]>.
+
+    Definition growth_tree_adder a n
+    : CavaExpr var << Vector (Vector Bit a) (2^(n+1)), Unit >> (Vector Bit (S (n + a)) ) :=
+    <[ \ v => !(dt_tree_fold' n a (Vector Bit) (growth_adder)) v  ]>.
+
+  End var.
+
+End notation.
+
+Open Scope kind_scope.
+Definition adder445 {cava: Cava}: 
+    << Vector Bit 4, Vector Bit 4 >> ~[cava]~> (Vector Bit 5) 
+  := to_arrow (fun var => unsigned_adder var 4 4 5).
+
+Lemma adder445_is_combinational: wf_combinational adder445.
+Proof. combinational_obvious. Qed.
+
+Definition adder88810 {cava: Cava}: 
+    << Vector Bit 8, Vector Bit 8, Vector Bit 8 >> ~[cava]~> (Vector Bit 10) 
+  := to_arrow (fun var => adder3 var 8 8 8).
+
+Lemma adder88810_is_combinational: wf_combinational adder88810.
+Proof. combinational_obvious. Qed.
+
+Lemma adder_tree_4_wf: forall (cava:Cava), wf_debrujin [] (desugar (tree_adder _ 4 1)).
+Proof. compute; tauto. Qed.
+Lemma adder_tree_8_wf: forall (cava:Cava), wf_debrujin [] (desugar (tree_adder _ 4 2)).
+Proof. compute; tauto. Qed.
+Lemma adder_tree_64_wf: forall (cava:Cava), wf_debrujin [] (desugar (tree_adder _ 4 5)).
+Proof. compute; tauto. Qed.
+
+Lemma growth_tree_8_wf: forall (cava:Cava), wf_debrujin [] (desugar (growth_tree_adder _ 4 2)).
+Proof. compute; tauto. Qed.
+
+Definition adder444_tree_4 {cava: Cava}: 
+  << Vector (Vector Bit 4) 4 >> ~[cava]~> (Vector Bit 4) 
+  := insert_rightmost_tt1 _ >>> Arrow.uncancelr >>> 
+  (closure_conversion' (object_decidable_equality:=decKind) []
+    (desugar (tree_adder _ 4 1))
+    (adder_tree_4_wf cava)).
+Definition adder444_tree_8 {cava: Cava}: 
+  << Vector (Vector Bit 4) 8 >> ~[cava]~> (Vector Bit 4) 
+  := insert_rightmost_tt1 _ >>> Arrow.uncancelr >>> 
+  closure_conversion' (object_decidable_equality:=decKind) []
+  ((desugar (tree_adder _ 4 2)))
+  (adder_tree_8_wf cava).
+Definition adder444_tree_64 {cava: Cava}: 
+  << Vector (Vector Bit 4) 64 >> ~[cava]~> (Vector Bit 4) 
+  := insert_rightmost_tt1 _ >>> Arrow.uncancelr >>> 
+  closure_conversion' (object_decidable_equality:=decKind) []
+  ((desugar (tree_adder _ 4 5)))
+  (adder_tree_64_wf  cava).
+
+Definition growth_tree_8 {cava: Cava}: 
+  << Vector (Vector Bit 4) 8>> ~[cava]~> (Vector Bit 7) 
+  := insert_rightmost_tt1 _ >>> Arrow.uncancelr >>> 
+  (closure_conversion' (object_decidable_equality:=decKind) []
+    (desugar (growth_tree_adder _ 4 2))
+    (growth_tree_8_wf cava)).
+
+Require Import Cava.Types.
+Require Import Cava.Netlist.
+
+Definition adder445_interface
+  := combinationalInterface "adder445"
+     (mkPort "a" (Kind.BitVec Kind.Bit 4), mkPort "b" (Kind.BitVec Kind.Bit 4))
+     (mkPort "sum" (Kind.BitVec Kind.Bit 5))
+     [].
+Definition adder88810_interface 
+  := combinationalInterface "adder88810"
+     (mkPort "a" (Kind.BitVec Kind.Bit 8), (mkPort "b" (Kind.BitVec Kind.Bit 8), mkPort "c" (Kind.BitVec Kind.Bit 8)))
+     (mkPort "sum" (Kind.BitVec Kind.Bit 10))
+     [].
+Definition adder444_tree_4_interface 
+  := combinationalInterface "adder444_tree_4"
+     (mkPort "vec" (Kind.BitVec (Kind.BitVec Kind.Bit 4) 4))
+     (mkPort "result" (Kind.BitVec Kind.Bit 4))
+     [].
+Definition adder444_tree_8_interface 
+  := combinationalInterface "adder444_tree_8"
+     (mkPort "vec" (Kind.BitVec (Kind.BitVec Kind.Bit 4) 8))
+     (mkPort "result" (Kind.BitVec Kind.Bit 4))
+     [].
+Definition adder444_tree_64_interface 
+  := combinationalInterface "adder444_tree_64"
+     (mkPort "vec" (Kind.BitVec (Kind.BitVec Kind.Bit 4) 64))
+     (mkPort "result" (Kind.BitVec Kind.Bit 4))
+     [].
+Definition growth_tree_8_interface 
+  := combinationalInterface "growth_tree_8"
+     (mkPort "vec" (Kind.BitVec (Kind.BitVec Kind.Bit 4) 8))
+     (mkPort "result" (Kind.BitVec Kind.Bit 7))
+     [].
+
+Lemma wf_adder445_io: wf_netlist_io (@adder445 NetlistCava).
+Proof. cbv [wf_netlist_io]; compute; tauto. Qed.
+Lemma wf_adder88810_io: wf_netlist_io (@adder88810 NetlistCava).
+Proof. cbv [wf_netlist_io]; compute; tauto. Qed.
+Lemma wf_adder_tree_4_io: wf_netlist_io (@adder444_tree_4 NetlistCava).
+Proof. cbv [wf_netlist_io]; compute; tauto. Qed.
+Lemma wf_adder_tree_8_io: wf_netlist_io (@adder444_tree_8 NetlistCava).
+Proof. cbv [wf_netlist_io]; compute; tauto. Qed.
+Lemma wf_adder_tree_64_io: wf_netlist_io (@adder444_tree_64 NetlistCava).
+Proof. cbv [wf_netlist_io]; compute; tauto. Qed.
+Lemma wf_growth_tree_8_io: wf_netlist_io (@growth_tree_8 NetlistCava).
+Proof. cbv [wf_netlist_io]; compute; tauto. Qed.
+
+Definition adder445_netlist :=
+  makeNetlist adder445_interface (arrow_netlist adder445 wf_adder445_io).
+
+Definition adder445_tb_inputs :=
+  map (fun '(x, y) => (N2Bv_sized 4 x, N2Bv_sized 4 y))
+  [(0, 0); (1, 2); (15, 1); (15, 15)]%N.
+
+Definition adder445_tb_expected_outputs
+  := map (fun i => evaluate adder445 adder445_is_combinational i) adder445_tb_inputs.
+
+Definition adder445_tb
+  := testBench "adder445_tb" adder445_interface
+     adder445_tb_inputs adder445_tb_expected_outputs.
+
+Definition adder88810_netlist :=
+  makeNetlist adder88810_interface (arrow_netlist adder88810 wf_adder88810_io).
+
+Definition adder88810_tb_inputs :=
+  map (fun '(x, y, z) => (N2Bv_sized 8 x, (N2Bv_sized 8 y, N2Bv_sized 8 z)))
+  [(17, 23, 95); (4, 200, 30); (255, 255, 200)]%N.
+
+Definition adder88810_tb_expected_outputs
+  := map (fun i => evaluate adder88810 adder88810_is_combinational i) adder88810_tb_inputs.
+
+Definition adder88810_tb
+  := testBench "adder88810_tb" adder88810_interface
+     adder88810_tb_inputs adder88810_tb_expected_outputs.
+
+Definition adder444_tree_4_netlist :=
+  makeNetlist adder444_tree_4_interface (arrow_netlist adder444_tree_4 wf_adder_tree_4_io).
+
+Definition adder444_tree_8_netlist :=
+  makeNetlist adder444_tree_8_interface (arrow_netlist adder444_tree_8 wf_adder_tree_8_io).
+
+Definition adder444_tree_64_netlist :=
+  makeNetlist adder444_tree_64_interface (arrow_netlist adder444_tree_64 wf_adder_tree_64_io).
+
+Definition adder444_tree_4_inputs :=
+  map (fun '(x, y, z, w) => [N2Bv_sized 4 x; N2Bv_sized 4 y; N2Bv_sized 4 z; N2Bv_sized 4 w]%vector)
+  [(0, 0, 0, 1); (1, 1, 1, 1); (1, 3, 5, 2); (15, 1, 1, 1)]%N.
+
+Lemma adder444_tree_4_is_combinational: wf_combinational adder444_tree_4.
+Proof. combinational_obvious. Qed.
+
+Definition adder444_tree_4_tb_expected_outputs
+  := map (fun i => evaluate adder444_tree_4 adder444_tree_4_is_combinational i) adder444_tree_4_inputs.
+
+Definition adder444_tree_4_tb
+  := testBench "adder444_tree_4_tb" adder444_tree_4_interface
+     adder444_tree_4_inputs adder444_tree_4_tb_expected_outputs.
+
+Definition growth_tree_8_netlist :=
+  makeNetlist growth_tree_8_interface (arrow_netlist growth_tree_8 wf_growth_tree_8_io).
+
+Definition growth_tree_8_inputs :=
+  map (Vector.map (N2Bv_sized 4))
+  [[0; 0; 0; 0; 0; 0; 0; 1]%vector %N
+  ;[1; 1; 1; 1; 1; 1; 1; 1]%vector %N
+  ;[1; 2; 3; 4; 5; 6; 7; 8]%vector %N
+  ;[15; 15; 15; 15; 15; 15; 15; 15]%vector %N
+  ].
+
+Lemma growth_tree_8_is_combinational: wf_combinational growth_tree_8.
+Proof. combinational_obvious. Qed.
+
+Definition growth_tree_8_tb_expected_outputs
+  := map (fun i => evaluate growth_tree_8 growth_tree_8_is_combinational i) growth_tree_8_inputs.
+
+Definition growth_tree_8_tb
+  := testBench "growth_tree_8_tb" growth_tree_8_interface
+     growth_tree_8_inputs growth_tree_8_tb_expected_outputs.
